$\bracket[\varphi_1\vee\varphi_2]=\left\{\begin{array}{ll}
    \bracket[(\epsilon\cdot\varphi_1)\cup\varphi_2] & if (q_1,\phi_1,p_1,a,s_1)\in\Delta_1 \\
    \bracket[\varphi_1\cup(\epsilon\cdot\varphi_2)] & if (q_2,\phi_2,p_2,a,s_2)\in\Delta_2 \\
    (Q_1\cup Q_2 \cup {s}\backslash\{s_1,s_2\},C_1\cup C_2,\Delta,\Sigma,s,F_1\cup F_2\backslash\{s_1,s_2\}) & otherwise \\
    \end{array}\right.
    $
    
    Where
    
    $\Delta_e=\{(q,\phi,p,a,q')|
    (q,\phi,p,a,q')\in\Delta_1\wedge q\neq s_1
    \vee
    (q,\phi,p,a,q')\in\Delta_2\wedge q\neq s_2\}$

    $\Delta_s=\{(s,\phi,p,a,q')|
    \exists. q (q,\phi,p,a,q')\in\Delta_1
    \vee    q (q,\phi,p,a,q')\in\Delta_2\}$

    $\Delta=\Delta_e\cup\Delta_s$
    \newline

    $\forall (q_1,\phi_1,p_1,a,q_1')\in\Delta_1\wedge q_1\neq s_1 \implies (q_1,\phi_1,p_1,a,q_1')\in\Delta$
    
    $\forall (q_2,\phi_2,p_2,a,q_2')\in\Delta_2\wedge q_2\neq s_2 \implies (q_2,\phi_2,p_2,a,q_2')\in\Delta$
    
    $\forall (s_1,\phi_1,p_1,a,q_1')\in\Delta_1\implies (s,\phi_1,p_1,a,q_1')\in\Delta$
    
    $\forall (s_2,\phi_2,p_2,a,q_2')\in\Delta_2\implies (s,\phi_2,p_2,a,q_2')\in\Delta$